Expand finite maps library.

src/mem/FiniteMaps.v
@@ -2,7 +2,26 @@ From Coq Require Import
   FSets.FMapAVL
   FSets.FSetAVL
   FSetProperties
-  FMapFacts.
+  FMapFacts
+  ZArith
+  Lia
+  List.
+
+From ExtLib Require Import
+  Structures.Monads
+  Structures.Functor
+  Structures.Applicative
+  Structures.Traversable
+  Structures.Foldable
+  Programming.Eqv.
+
+From Mem Require Import Tactics.
+
+Import ListNotations.
+Import MonadNotation.
+Import FunctorNotation.
+Import ApplicativeNotation.
+Open Scope monad.
 
 Module IM := FMapAVL.Make(Coq.Structures.OrderedTypeEx.Z_as_OT).
 Module IS := FSetAVL.Make(Coq.Structures.OrderedTypeEx.Z_as_OT).
@@ -50,3 +69,717 @@ Proof.
   apply IS.add_2; auto.
   apply IS.mem_2; auto.
 Qed.
+
+#[global] Coercion is_true : bool >-> Sortclass.
+
+Section Map_Operations.
+
+  (** ** Finite maps
+      We use finite maps in several place of the memory model. We rely on the AVL implementation from the standard library.
+      We redefine locally the operations we use and their axiomatisation as the interface exposed by the standard library
+      tends to leak out the [Raw] underlying implementation, and feels overall tedious to use.
+   *)
+
+  (* Polymorphic type of maps indexed by [Z] *)
+  Definition IntMap := IM.t.
+
+  Definition add {a} k (v:a) := IM.add k v.
+  Definition delete {a} k (m:IntMap a) := IM.remove k m.
+  Definition member {a} k (m:IntMap a) := IM.mem k m.
+  Definition lookup {a} k (m:IntMap a) := IM.find k m.
+  Definition empty {a} := @IM.empty a.
+
+  Definition add_with {a b} k (v:a) (def : a -> b) (merge : a -> b -> b) (m:IntMap b) :=
+    match IM.find k m with
+    | None => add k (def v) m
+    | Some elt =>
+        add k (merge v elt) m
+    end.
+
+  (* We use two notions of equivalence of maps depending on the type of objects stored.
+       When we can get away with Leibniz's equality over the return type, we simply use
+       [Equal] that implements extensional equality (and equality of domains).
+       When the domain of value itself has a non-trivial notion of equivalence, we use [Equiv]
+       which relax functional equivalence up-to this relation.
+   *)
+  Definition Equal {a} : IntMap a -> IntMap a -> Prop :=
+    fun m m' => forall k, lookup k m = lookup k m'.
+  Definition Equiv {a} (R : a -> a -> Prop) : IntMap a -> IntMap a -> Prop :=
+    fun m m' =>
+      (forall k, member k m <-> member k m') /\
+      (forall k e e', lookup k m = Some e -> lookup k m' = Some e' -> R e e').
+
+  (* Extends the map with a list of pairs key/value.
+     Note: additions start from the end of the list, so in case of duplicate
+     keys, the binding in the front will shadow though in the back.
+   *)
+  Fixpoint add_all {a} ks (m:IntMap a) :=
+    match ks with
+    | [] => m
+    | (k,v) :: tl => add k v (add_all tl m)
+    end.
+
+  (* Extends the map with the bindings {(i,v_1) .. (i+n-1, v_n)} for [vs ::= v_1..v_n] *)
+  Fixpoint add_all_index {a} vs (i:Z) (m:IntMap a) :=
+    match vs with
+    | [] => m
+    | v :: tl => add i v (add_all_index tl (i+1) m)
+    end.
+
+  (* Takes the join of two maps, favoring the first one over the intersection of their domains *)
+  Definition union {a} (m1 : IntMap a) (m2 : IntMap a)
+    := IM.map2 (fun mx my =>
+                  match mx with | Some x => Some x | None => my end) m1 m2.
+
+  (* TODO : Move the three following functions *)
+  Fixpoint max_default (l:list Z) (x:Z) :=
+    match l with
+    | [] => x
+    | h :: tl =>
+      max_default tl (if h >? x then h else x)%Z
+    end.
+
+  Definition maximumBy {A} (leq : A -> A -> bool) (def : A) (l : list A) : A :=
+    fold_left (fun a b => if leq a b then b else a) l def.
+
+  Definition maximumBy_Z_le_def :
+    forall def l e,
+      (e <=? def ->
+       e <=? maximumBy Z.leb def l)%Z.
+  Proof using.
+    intros def l.
+    revert def.
+    induction l; intros def e LE.
+    - cbn; auto.
+    - cbn. destruct (def <=? a)%Z eqn:Hdef.
+      + apply IHl.
+        eapply Zle_bool_trans; eauto.
+      + apply IHl; auto.
+  Qed.
+
+  Definition maximumBy_Z_def :
+    forall def l,
+      (def <=? maximumBy Z.leb def l)%Z.
+  Proof using.
+    intros def l.
+    apply maximumBy_Z_le_def; eauto.
+    apply Z.leb_refl.
+  Qed.
+
+  Definition maximumBy_Z_correct :
+    forall def (l : list Z),
+    forall a, In a l -> Z.leb a (maximumBy Z.leb def l).
+  Proof using.
+    intros def l.
+    revert def.
+    induction l as [|x xs];
+      intros def a IN;
+      inversion IN.
+    - subst; cbn.
+      apply maximumBy_Z_le_def.
+      destruct (def <=? a)%Z eqn:LE.
+      + apply Z.leb_refl.
+      + rewrite Z.leb_gt in LE.
+        apply Z.leb_le.
+        lia.
+    - subst; cbn; apply IHxs; auto.
+  Qed.
+
+  Definition is_some {A} (o : option A) :=
+    match o with
+    | Some x => true
+    | None => false
+    end.
+
+  Fixpoint IM_raw_greatest_key {A} (m : IM.Raw.tree A) : option Z
+    := match m with
+       | IM.Raw.Leaf _ => None
+       | IM.Raw.Node l k _ (@IM.Raw.Leaf _) _ =>
+           Some k
+       | IM.Raw.Node l k _ r _ =>
+           IM_raw_greatest_key r
+       end.
+
+  Definition IM_greatest_key {A} (m : IM.t A) : option Z
+    := IM_raw_greatest_key (IM.this m).
+
+  Definition next_key {A} (m : IntMap A) : Z
+    := match IM_greatest_key m with
+       | Some k => 1 + k
+       | None => 0
+       end.
+
+  Definition next_key_old {A} (m : IntMap A) : Z
+    := let keys := map fst (IM.elements m) in
+       1 + maximumBy Z.leb (-1)%Z keys.
+
+  Lemma next_key_old_gt_0 :
+    forall {A} (m : IntMap A),
+      (next_key_old m >= 0)%Z.
+  Proof using.
+    intros A m.
+    unfold next_key_old.
+    pose proof maximumBy_Z_def (-1) (map fst (IM.elements (elt:=A) m)).
+    apply Zle_is_le_bool in H.
+    lia.
+  Qed.
+
+  Lemma IM_greatest_key_none' :
+    forall {A} (m : IM.t A), IM.Empty m -> IM_greatest_key m = None.
+  Proof.
+    intros A m H.
+    induction m; cbn in *.
+    induction this; cbn in *; auto.
+    - exfalso; eapply H.
+      cbn.
+      constructor; reflexivity.
+  Qed.
+
+  Lemma IM_greatest_key_none'' :
+    forall {A} (m : IM.t A), IM_greatest_key m = None -> IM.Empty m.
+  Proof.
+    intros A m H.
+    induction m; cbn in *.
+    induction this; cbn in *; auto.
+    - intros k e CONTRA.
+      inversion CONTRA.
+    - exfalso.
+      destruct (IM_raw_greatest_key this2) eqn:THIS2.
+      + break_match_hyp_inv.
+      + break_match_hyp_inv.
+        inv is_bst.
+        specialize (IHthis2 H5 eq_refl).
+        eapply IHthis2.
+        constructor; reflexivity.
+  Qed.
+
+  Lemma IM_greatest_key_none :
+    forall {A} (m : IM.t A), IM_greatest_key m = None <-> IM.Empty m.
+  Proof.
+    intros A m.
+    split; intros H.
+    + apply IM_greatest_key_none''; auto.
+    + apply IM_greatest_key_none'; auto.
+  Qed.
+
+  Lemma IM_greatest_key_In :
+    forall {A} (m : IM.t A) gk,
+      IM_greatest_key m = Some gk -> IM.In gk m.
+  Proof.
+    intros A m.
+    intros gk H.
+    apply F.in_find_iff.
+    revert gk H.
+    destruct m; cbn in *.
+    induction this; intros gk GK.
+    - cbn in *. inv GK.
+    - rename k into current_key.
+      cbn.
+      (* gk is the greatest key. It should be larger than current_key *)
+      cbn in GK.
+      pose proof is_bst as is_bst2.
+      inv is_bst.
+      destruct (IM_raw_greatest_key this2) eqn:THIS2;
+        destruct this2; inv GK.
+      + (* At a leaf eq *)
+        break_match; cbn in *;
+          solve
+            [ red in l; lia
+            | discriminate
+            ].
+      + (* Not at a leaf... *)
+        pose proof H5.
+        eapply IHthis2 in H5; eauto.
+        eapply IM.Raw.Proofs.find_in_iff in H5; eauto.
+
+        red in H7.
+        apply H7 in H5.
+
+        break_match; cbn in *;
+          try solve
+            [ red in l; lia
+            | discriminate
+            ].
+
+        apply IHthis2; auto.
+      + break_match; cbn in *;
+          solve
+            [ red in l; lia
+            | discriminate
+            ].
+  Qed.
+
+  Lemma IM_greatest_key_In' :
+    forall {A} (m : IM.t A) k,
+      IM.In k m ->
+      exists gk, IM_greatest_key m = Some gk.
+  Proof.
+    intros A m k IN.
+    destruct (IM_greatest_key m) eqn:GK.
+    exists z; auto.
+
+    apply F.in_find_iff in IN.
+    destruct (IM.find (elt:=A) k m) eqn:FIND; try contradiction.
+    apply F.find_mapsto_iff in FIND.
+    apply IM_greatest_key_none in FIND; try contradiction; auto.
+  Qed.
+
+  Lemma IM_greatest_key_lt :
+    forall {A} (m : IM.t A) gk,
+      IM_greatest_key m = Some gk -> IM.Raw.lt_tree (1 + gk) (IM.this m).
+  Proof.
+    intros A m.
+    destruct m; cbn in *.
+    induction this; intros gk GK.
+    - cbn in *. inv GK.
+    - rename k into current_key.
+      cbn.
+      (* gk is the greatest key. It should be larger than current_key *)
+      cbn in GK.
+      pose proof is_bst as is_bst2.
+      inv is_bst.
+      destruct (IM_raw_greatest_key this2) eqn:THIS2;
+        destruct this2; inv GK.
+      + (* At a leaf eq *)
+        break_match; cbn in *;
+          solve
+            [ red in l; lia
+            | discriminate
+            ].
+      + (* Not at a leaf... *)
+        pose proof H5.
+        eapply IHthis2 in H5; eauto.
+        red.
+        intros y H0.
+        inv H0.
+        * (* Root *)
+          red in H5.
+          specialize (H5 k).
+          forward H5.
+          constructor; auto.
+          specialize (H7 k).
+          forward H7.
+          constructor; auto.
+          cbn in H7.
+          lia.
+        * (* Left *)
+          red in H6.
+          specialize (H6 y H2).
+          red in H5.
+          specialize (H5 k).
+          forward H5.
+          constructor; auto.
+          specialize (H7 k).
+          forward H7.
+          constructor; auto.
+          cbn in H7.
+          lia.
+        * (* Right *)
+          red in H5.
+          specialize (H5 y H2).
+          auto.
+      + red.
+        intros y H.
+        assert (gk < 1 + gk)%Z by lia.
+        inv H; auto.
+        * apply H6 in H2.
+          cbn in *; lia.
+        * inv H2.
+  Qed.
+
+
+  Lemma IM_raw_greatest_key_lr :
+    forall {elt} m k (e : elt) l t r kl kr,
+      IM.this m = (IM.Raw.Node l k e r t) ->
+      IM_raw_greatest_key l = Some kl ->
+      IM_raw_greatest_key r = Some kr ->
+      (kl < kr)%Z.
+  Proof.
+    intros elt m k e l t r kl kr NODE GL GR.
+    destruct m.
+    cbn in *.
+    inv is_bst.
+    inv H.
+    inv H3.
+
+    unfold IM.Raw.gt_tree in *.
+    unfold IM.Raw.lt_tree in *.
+
+    assert (IM_greatest_key (@IM.Bst elt l H) = Some kl) as GL' by (cbn; auto).
+    assert (IM_greatest_key (@IM.Bst elt r H0) = Some kr) as GR' by (cbn; auto).
+
+    apply IM_greatest_key_In in GL', GR'.
+    unfold IM.In in *.
+    apply IM.Raw.Proofs.In_alt in GL', GR'.
+    apply H2 in GR'.
+    apply H1 in GL'.
+
+    lia.
+  Qed.
+
+  Lemma next_key_correct :
+    forall {A} (m : IM.t A) (a : Z),
+      IM.In a m ->
+      (a < next_key m)%Z.
+  Proof.
+    intros A m a IN.
+    pose proof IN as GK.
+    unfold next_key.
+    eapply IM_greatest_key_In' in GK.
+    destruct GK as (gk & GK).
+    rewrite GK.
+    apply IM_greatest_key_lt in GK.
+    red in GK.
+    specialize (GK a).
+    destruct m; cbn in IN.
+    unfold IM.In in IN.
+    apply IM.Raw.Proofs.In_alt in IN.
+    apply GK in IN.
+    auto.
+  Qed.
+
+  Lemma MapsTo_inj : forall {a} k v v' (m : IntMap a),
+    IM.MapsTo k v m ->
+    IM.MapsTo k v' m ->
+    v = v'.
+  Proof using.
+    intros.
+    apply IM.find_1 in H; apply IM.find_1 in H0.
+    rewrite H0 in H; inversion H.
+    reflexivity.
+  Qed.
+
+    (** ** [member]/[lookup] interaction
+        Keys are in the domain if and only if they lead to values when looked-up
+   *)
+  Lemma member_lookup {a} : forall k (m : IntMap a),
+      member k m -> exists v, lookup k m = Some v.
+  Proof using.
+    unfold member,lookup in *.
+    intros * IN.
+    apply IM.Raw.Proofs.mem_2, IM.Raw.Proofs.In_MapsTo in IN.
+    destruct IN as [v IN].
+    exists v.
+    apply IM.Raw.Proofs.find_1; eauto.
+    apply IM.is_bst.
+  Qed.
+
+  Lemma lookup_member {a} : forall k v(m : IntMap a),
+      lookup k m = Some v -> member k m .
+  Proof using.
+    unfold member,lookup in *.
+    intros * IN.
+    apply IM.Raw.Proofs.mem_1; [apply IM.is_bst |].
+    apply IM.Raw.Proofs.find_2 in IN; eauto.
+    eapply IM.Raw.Proofs.MapsTo_In; eauto.
+  Qed.
+
+  (** ** [add]/[lookup] interaction
+        Lookups look up the lastly added value
+   *)
+  Lemma lookup_add_eq : forall {a} k x (m : IntMap a),
+      lookup k (add k x m) = Some x.
+  Proof using.
+    intros.
+    unfold lookup, add.
+    apply IM.find_1, IM.add_1; auto.
+  Qed.
+
+  Lemma lookup_add_ineq : forall {a} k k' x (m : IntMap a),
+      k <> k' ->
+      lookup k (add k' x m) = lookup k m.
+  Proof using.
+    intros.
+    unfold lookup, add.
+    match goal with
+      |- ?x = ?y => destruct x eqn:EQx,y eqn:EQy;
+                    try apply IM.find_2,IM.add_3 in EQx;
+                    try apply IM.find_2 in EQy
+    end; auto.
+    eapply MapsTo_inj in EQx; eauto; subst; eauto.
+    apply IM.find_1 in EQx; rewrite EQx in EQy; inversion EQy.
+    cbn in *.
+    apply IM.Raw.Proofs.not_find_iff in EQx; [| apply IM.Raw.Proofs.add_bst, IM.is_bst].
+    exfalso; apply EQx, IM.Raw.Proofs.add_in.
+    right.
+    unfold IM.MapsTo in *.
+    eapply IM.Raw.Proofs.MapsTo_In,EQy.
+  Qed.
+
+  (** ** [add]/[member] interaction
+        Added keys are a member of the map
+   *)
+  Lemma member_add_eq {a}: forall k v (m: IntMap a),
+      member k (add k v m).
+  Proof using.
+    intros.
+    cbn.
+    apply IM.Raw.Proofs.mem_1.
+    apply IM.Raw.Proofs.add_bst, IM.is_bst.
+    rewrite IM.Raw.Proofs.add_in; auto.
+  Qed.
+
+  Lemma member_add_ineq {a}: forall k k' v (m: IntMap a),
+      k <> k' ->
+      member k (add k' v m) <-> member k m.
+  Proof using.
+    intros.
+    cbn. split.
+    - intros IN; apply IM.Raw.Proofs.mem_2 in IN.
+      rewrite IM.Raw.Proofs.add_in in IN.
+      destruct IN as [-> | IN]; [contradiction H; auto | ].
+      apply IM.Raw.Proofs.mem_1; [apply IM.is_bst | auto].
+    - intros IN.
+      apply IM.Raw.Proofs.mem_1.
+      apply IM.Raw.Proofs.add_bst, IM.is_bst.
+      rewrite IM.Raw.Proofs.add_in; right; auto.
+      apply IM.Raw.Proofs.mem_2 in IN; auto.
+  Qed.
+
+  Lemma member_add_preserved {a}: forall k k' v (m: IntMap a),
+      member k m ->
+      member k (add k' v m).
+  Proof using.
+    intros k k' v m H.
+    cbn in *.
+    apply IM.Raw.Proofs.mem_1.
+    apply IM.Raw.Proofs.add_bst, IM.is_bst.
+    rewrite IM.Raw.Proofs.add_in; auto.
+    right. apply IM.Raw.Proofs.mem_2.
+    apply H.
+  Qed.
+
+  (** ** Equivalences
+        Both notions of equivalence of maps that we manipulate are indeed equivalences
+        (assuming the relation on values is itself an equivalence for [Equiv]).
+   *)
+  #[global] Instance Equal_Equiv {a}: Equivalence (@Equal a).
+  Proof using.
+    split.
+    - repeat intro; reflexivity.
+    - repeat intro.
+      symmetry; apply H.
+    - intros ? ? ? EQ1 EQ2 ?.
+      etransitivity; eauto.
+  Qed.
+
+  #[global] Instance Equiv_Equiv {a} {r: a -> a -> Prop} {rE : Equivalence r} : Equivalence (Equiv r).
+  Proof using.
+    split.
+    - intros ?; split.
+      intros k; reflexivity.
+      intros * LU1 LU2; rewrite LU1 in LU2; inversion LU2; reflexivity.
+    - intros ? ? [DOM EQ]; split.
+      intros ?; split; intros ?; apply DOM; auto.
+      intros; symmetry; eapply EQ; eauto.
+    - intros ? ? ? [DOM1 EQ1] [DOM2 EQ2]; split.
+      intros ?; split; intros ?.
+      apply DOM2,DOM1; auto.
+      apply DOM1,DOM2; auto.
+      intros ? ? ? LU1 LU2.
+      generalize LU1; intros LU3; apply lookup_member,DOM1,member_lookup in LU3.
+      destruct LU3 as [e'' LU3].
+      transitivity e''.
+      eapply EQ1; eauto.
+      eapply EQ2; eauto.
+  Qed.
+
+  #[global] Instance Proper_lookup {a} k: Proper (@Equal a ==> Logic.eq) (lookup k).
+  Proof using.
+    repeat intro.
+    apply H.
+  Qed.
+
+  #[global] Instance Proper_add {a} : Proper (Logic.eq ==> Logic.eq ==> Equal ==> Equal) (@add a).
+  Proof using.
+    repeat intro; subst.
+    destruct (Z.eq_dec k y); [subst; rewrite 2 lookup_add_eq; auto | rewrite 2 lookup_add_ineq; auto].
+  Qed.
+
+  (** ** [add]/[add]
+        Consecutive extensions of the map either commute or erase the oldest one.
+   *)
+  Lemma add_add : forall {a} off b1 b2 (m : IM.t a),
+      Equal (add off b2 (add off b1 m)) (add off b2 m).
+  Proof using.
+    intros; intro key; cbn.
+    rewrite IM.Raw.Proofs.add_find; [| apply IM.Raw.Proofs.add_bst, IM.is_bst].
+    rewrite IM.Raw.Proofs.add_find; [| apply  IM.is_bst].
+    rewrite IM.Raw.Proofs.add_find; [| apply  IM.is_bst].
+    flatten_goal; auto.
+  Qed.
+
+  Lemma Equiv_add_add : forall {a} {r: a -> a -> Prop} {rR: Reflexive r},
+      forall k v1 v2 (m: IM.t a),
+        Equiv r (add k v2 (add k v1 m)) (add k v2 m).
+  Proof using.
+    intros; split.
+    - intros key.
+      destruct (Z.eq_dec key k).
+      + subst; rewrite 2 member_add_eq; reflexivity.
+      + subst; rewrite 3 member_add_ineq; auto; reflexivity.
+    - intros key v v' LU1 LU2; cbn.
+      destruct (Z.eq_dec key k).
+      + subst; rewrite lookup_add_eq in LU1, LU2; inv LU1; inv LU2.
+        reflexivity.
+      + subst; rewrite lookup_add_ineq in LU1, LU2; auto; rewrite lookup_add_ineq in LU1; auto.
+        rewrite LU1 in LU2; inv LU2.
+        reflexivity.
+  Qed.
+
+  Lemma add_add_ineq : forall {a} k1 k2 v1 v2 (m : IM.t a),
+      k1 <> k2 ->
+      Equal (add k2 v2 (add k1 v1 m)) (add k1 v1 (add k2 v2 m)).
+  Proof using.
+    intros; intro key; cbn.
+    rewrite IM.Raw.Proofs.add_find; [| apply IM.Raw.Proofs.add_bst, IM.is_bst].
+    rewrite IM.Raw.Proofs.add_find; [| apply  IM.is_bst].
+    rewrite IM.Raw.Proofs.add_find; [| apply IM.Raw.Proofs.add_bst, IM.is_bst].
+    rewrite IM.Raw.Proofs.add_find; [| apply  IM.is_bst].
+    pose proof (IM.Raw.Proofs.MX.eqb_alt key k2).
+    flatten_goal; auto.
+    pose proof (IM.Raw.Proofs.MX.eqb_alt key k1).
+    flatten_goal; auto.
+    unfold IM.Raw.Proofs.MX.eqb in *.
+    flatten_hyp H0.
+    flatten_hyp H1.
+    subst; contradiction H; auto.
+    inv H1.
+    inv H0.
+  Qed.
+
+  Lemma key_in_range_or_not_aux {a} : forall (k z : Z) (l : list a),
+      ({z <= k <= z + Zlength l - 1} + {k < z} + {k >= z + Zlength l})%Z.
+  Proof using.
+    induction l as [| x l IH]; intros.
+    - cbn; rewrite Z.add_0_r.
+      destruct (Z_lt_ge_dec k z); [left; right; auto | right; lia].
+    - rewrite Zlength_cons, <- Z.add_1_r.
+      destruct IH as [[IH | IH] | IH].
+      + left; left; lia.
+      + left; right; lia.
+      + destruct (Z.eq_dec k (z + Zlength l)).
+        * subst; left; left; rewrite Zlength_correct; lia.
+        * right; lia.
+  Qed.
+
+  Lemma key_in_range_or_not {a} : forall (k z : Z) (l : list a),
+      ({z <= k <= z + Zlength l - 1} + {k < z \/ k >= z + Zlength l})%Z.
+  Proof using.
+    intros; destruct (@key_in_range_or_not_aux _ k z l) as [[? | ?] | ?]; [left; auto | right; auto | right; auto].
+  Qed.
+
+  Fixpoint IM_find_many {A} (xs : list Z) (im : IntMap A) : option (list A)
+    := match xs with
+       | [] => ret []
+       | (x::xs) =>
+         elt  <- IM.find x im;;
+         elts <- IM_find_many xs im;;
+         ret (elt :: elts)
+       end.
+
+  (* Merge taking the latter arguments' values if duplicates.
+   Unclear if IM.Raw.merge would have this property.
+   *)
+  Definition IM_merge {a} (m1 : IM.Raw.t a) (m2 : IM.Raw.t a) : IM.Raw.t a
+    := IM.Raw.fold (IM.Raw.add (elt:=a)) m2 m1.
+
+  Definition IM_Refine {a b} (R : a -> b -> Prop) : IntMap a -> IntMap b -> Prop :=
+    fun m m' =>
+      (forall k, member k m <-> member k m') /\
+        (forall k e e', lookup k m = Some e -> lookup k m' = Some e' -> R e e').
+
+  Lemma IM_Refine_empty :
+    forall {R1 R2} (R1R2 : R1 -> R2 -> Prop),
+      IM_Refine R1R2 (IM.empty R1) (IM.empty R2).
+  Proof.
+    intros R1 R2 R1R2.
+    split.
+    - intros k.
+      split; intros MEM;
+        inv MEM.
+    - intros k e e' L1 L2.
+      inv L1.
+  Qed.
+
+  Lemma IM_Refine_add :
+    forall {R1 R2} (R1R2 : R1 -> R2 -> Prop) m1 m2 k x y
+      (REF : IM_Refine R1R2 m1 m2)
+      (RXY : R1R2 x y),
+      IM_Refine R1R2 (add k x m1) (add k y m2).
+  Proof.
+    intros R1 R2 R1R2 m1 m2 k x y REF RXY.
+    split.
+    - intros k0.
+      destruct (Z.eq_dec k k0) eqn:K; subst.
+      + split; intros MEM; apply member_add_eq.
+      + split; intros MEM; apply member_add_ineq;
+          apply member_add_ineq in MEM; eauto;
+          apply REF; auto.
+    - intros k0 e e' L L'.
+      destruct (Z.eq_dec k k0) eqn:K; subst.
+      + rewrite lookup_add_eq in L.
+        rewrite lookup_add_eq in L'.
+        inv L; inv L'; auto.
+      + rewrite lookup_add_ineq in L; eauto.
+        rewrite lookup_add_ineq in L'; eauto.
+        eapply REF; eauto.
+  Qed.
+End Map_Operations.
+
+Definition traverseWithKeyRaw {t} `{Applicative t} {a b} (f : IM.Raw.key -> a -> t b) (m : IM.Raw.t a) : t (IM.Raw.t b)
+  :=
+  let fix go x :=
+    match x with
+    | IM.Raw.Leaf _ => pure (IM.Raw.Leaf _)
+    | IM.Raw.Node l k v r h =>
+        if Z.eqb 1%Z h
+        then (fun v' => IM.Raw.Node (IM.Raw.Leaf _) k v' (IM.Raw.Leaf _) 1%Z) <$> f k v
+        else (fun l' v' r' => IM.Raw.Node l' k v' r' h) <$> go l <*> f k v <*> go r
+    end
+  in
+  go m.
+
+#[global] Instance Traversable_RawIntMap : Traversable IM.Raw.t.
+split.
+intros F Ap A B X X0.
+eapply traverseWithKeyRaw.
+intros k.
+apply X.
+apply X0.
+Defined.
+
+Definition traverseWithKey {t} `{Applicative t} {a b} (f : IM.key -> a -> t b) (m : IM.t a) : t (IM.t b).
+  eapply @IM.fold.
+  3: apply (pure (IM.empty _)).
+  2: apply m.
+  - intros k e acc.
+    refine (let res := f k e in _).
+    eapply ap.
+    2: apply acc.
+    eapply fmap.
+    2: apply res.
+    apply (IM.add k).
+Defined.
+
+#[global] Instance Traversable_IntMap : Traversable IntMap.
+split.
+intros F Ap A B X X0.
+eapply traverseWithKey.
+intros k.
+apply X.
+apply X0.
+Defined.
+
+Import Monoid.
+#[global] Instance Foldable_IS : Foldable IS.t Z.
+split.
+intros m M conv s.
+apply (IS.fold (fun k acc => monoid_plus M (conv k) acc) s (monoid_unit M)).
+Defined.
+
+#[global] Instance Foldable_IM_Raw {a} : Foldable (IM.Raw.t a) Z.
+split.
+intros m M conv s.
+apply (IM.Raw.fold (fun k _ acc => monoid_plus M (conv k) acc) s (monoid_unit M)).
+Defined.
